
$$\begin{array}{l c r}{{\mathbf{e}^{n}=\sum\limits_{n=0}^{∞}\frac{x^{n}}{n!}=1+x+{\frac{x^{2}}{2!}}+\cdots+{\frac{x^{n}}{n!}}+\cdots,\scriptstyle-\infty<x<+\infty.}}\\ {{\qquad\qquad}}&{{}}\end{array}$$

$${\frac{1}{1+x}}={\sum\limits_{n=0}^{∞}(-1)^{n}x^{n}}=1-x+x^{2}-x^{3}+\cdots+(-1)^{n}x^{n}+\cdots{,-1<x<1}$$

$${\frac{1}{1-x}}={\sum\limits_{n=0}^{∞}x^{n}}=1+x+x^{2}+\cdots+x^{n}+\cdots{,-1<x<1}$$

$$\ln(1+x)={\sum\limits_{n=0}^{∞}(-1)^{n}}\frac{x^{2n+1}}{(2n+1)!}=x-{\frac{x^{2}}{2}}+{\frac{x^{3}}{3}}-{\frac{x^{4}}{4}}+\cdots+(-1)^{n-1}\,{\frac{x^{n}}{n}}+\cdots,\scriptstyle-1<x<+1.$$

$${\sin x=\sum\limits_{n=0}^{∞}(-1)^{n}\frac{x^{2n+1}}{(2n+1)!}=x-{\frac{x^{3}}{3!}}+{\frac{x^{5}}{5!}}-{\frac{x^{7}}{7!}}+\cdots+\cdots+(-1)^{n}\,{\frac{x^{2n+1}}{(2n+1)!}}+\cdots,\scriptstyle-\infty<x<+\infty.}$$

$${cosx=\sum\limits_{n=0}^{∞}(-1)^{n}\frac{x^{2n}}{(2n)!}}={1-{\frac{x^{2}}{2!}}+{\frac{x^{4}}{4!}}-{\frac{x^{6}}{6!}}+\cdots+(-1)^{n}\frac{x^{2n}}{(2n)!}+\cdots,\scriptstyle-\infty<x<+\infty.}$$

$$(1+x)^{\alpha}=\textstyle{1+\alpha x+{\frac{\alpha(\alpha-1)}{2!}}x^{2}+\cdots+\frac{\alpha(\alpha-1)...(\alpha-n+1)}{n!}x^n+\cdots,}$$
$${{(x\in(-1,1),\ \alpha\leq-1;x\in(-1,\ 1],\ -1<\alpha\leq0;x\in[-1,1],\alpha>0,\alpha\notin\mathbb{N}}}$$

$${\mathrm{tan}}x=x+\frac{1}{3}\,x^{3}+\cdots~.$$

$${arcsin x}=x+{\frac{1}{6}}\,x^{3}+\cdots$$

$$arctanx=x+{\frac{1}{3}}\,x^{3}+\cdots$$
